Strata/DL/Lambda/IntBoolFactory.lean
@@ -19,148 +19,147 @@ open LExpr LTy
 
 section IntBoolFactory
 
-def unaryOp [Coe String Ident]
-            (n : Ident)
+variable {T : LExprParams} [Coe String T.Identifier]
+
+def unaryOp (n : T.Identifier)
             (ty : LMonoTy)
-            (ceval : Option (LExpr LMonoTy Ident → List (LExpr LMonoTy Ident) → LExpr LMonoTy Ident)) : LFunc Ident :=
+            (ceval : Option (LExpr T.mono → List (LExpr T.mono) → LExpr T.mono)) : LFunc T :=
   { name := n,
     inputs := [("x", ty)],
     output := ty,
     concreteEval := ceval }
 
-def binaryOp [Coe String Ident]
-             (n : Ident)
+def binaryOp (n : T.Identifier)
              (ty : LMonoTy)
-             (ceval : Option (LExpr LMonoTy Ident → List (LExpr LMonoTy Ident) → LExpr LMonoTy Ident)) : LFunc Ident :=
+             (ceval : Option (LExpr T.mono → List (LExpr T.mono) → LExpr T.mono)) : LFunc T :=
   { name := n,
     inputs := [("x", ty), ("y", ty)],
     output := ty,
     concreteEval := ceval }
 
-def binaryPredicate [Coe String Ident]
-                    (n : Ident)
+def binaryPredicate (n : T.Identifier)
                     (ty : LMonoTy)
-                    (ceval : Option (LExpr LMonoTy Ident → List (LExpr LMonoTy Ident) → LExpr LMonoTy Ident)) : LFunc Ident :=
+                    (ceval : Option (LExpr T.mono → List (LExpr T.mono) → LExpr T.mono)) : LFunc T :=
   { name := n,
     inputs := [("x", ty), ("y", ty)],
     output := .bool,
     concreteEval := ceval }
 
-def unOpCeval  {Identifier : Type} (InTy OutTy : Type) [ToString OutTy]
-                (cevalInTy : (LExpr LMonoTy Identifier) → Option InTy) (op : InTy → OutTy)
+def unOpCeval (InTy OutTy : Type) [ToString OutTy]
+                (cevalInTy : (LExpr T.mono) → Option InTy) (op : InTy → OutTy)
                 (ty : LMonoTy) :
-                (LExpr LMonoTy Identifier) → List (LExpr LMonoTy Identifier) → (LExpr LMonoTy Identifier) :=
+                (LExpr T.mono) → List (LExpr T.mono) → (LExpr T.mono) :=
   (fun e args => match args with
    | [e1] =>
      let e1i := cevalInTy e1
      match e1i with
-     | some x => (LExpr.const (toString (op x)) ty)
+     | some x => (LExpr.const e1.metadata (toString (op x)) ty)
      | _ => e
    | _ => e)
 
-def binOpCeval {Identifier : Type} (InTy OutTy : Type) [ToString OutTy]
-                (cevalInTy : (LExpr LMonoTy Identifier) → Option InTy) (op : InTy → InTy → OutTy)
+def binOpCeval (InTy OutTy : Type) [ToString OutTy]
+                (cevalInTy : (LExpr T.mono) → Option InTy) (op : InTy → InTy → OutTy)
                 (ty : LMonoTy) :
-                (LExpr LMonoTy Identifier) → List (LExpr LMonoTy Identifier) → (LExpr LMonoTy Identifier) :=
+                (LExpr T.mono) → List (LExpr T.mono) → (LExpr T.mono) :=
   (fun e args => match args with
    | [e1, e2] =>
      let e1i := cevalInTy e1
      let e2i := cevalInTy e2
      match e1i, e2i with
-     | some x, some y => (LExpr.const (toString (op x y)) ty)
+     | some x, some y => (LExpr.const e1.metadata (toString (op x y)) ty)
      | _, _ => e
    | _ => e)
 
 -- We hand-code a denotation for `Int.Div` to leave the expression
 -- unchanged if we have `0` for the denominator.
-def cevalIntDiv (e : LExpr LMonoTy Ident) (args : List (LExpr LMonoTy Ident)) : LExpr LMonoTy Ident :=
+def cevalIntDiv (e : LExpr T.mono) (args : List (LExpr T.mono)) : LExpr T.mono :=
   match args with
   | [e1, e2] =>
-    let e1i := LExpr.denoteInt e1
-    let e2i := LExpr.denoteInt e2
+    let e1i := LExpr.denoteInt T e1
+    let e2i := LExpr.denoteInt T e2
     match e1i, e2i with
     | some x, some y =>
-      if y == 0 then e else (.const (toString (x / y)) (.some .int))
+      if y == 0 then e else (.const e.metadata (toString (x / y)) (.some .int))
     | _, _ => e
   | _ => e
 
 -- We hand-code a denotation for `Int.Mod` to leave the expression
 -- unchanged if we have `0` for the denominator.
-def cevalIntMod (e : LExpr LMonoTy Ident) (args : List (LExpr LMonoTy Ident)) : LExpr LMonoTy Ident :=
+def cevalIntMod (e : LExpr T.mono) (args : List (LExpr T.mono)) : LExpr T.mono :=
   match args with
   | [e1, e2] =>
-    let e1i := LExpr.denoteInt e1
-    let e2i := LExpr.denoteInt e2
+    let e1i := LExpr.denoteInt T e1
+    let e2i := LExpr.denoteInt T e2
     match e1i, e2i with
     | some x, some y =>
-      if y == 0 then e else (.const (toString (x % y)) (.some .int))
+      if y == 0 then e else (.const e.metadata (toString (x % y)) (.some .int))
     | _, _ => e
   | _ => e
 
 /- Integer Arithmetic Operations -/
 
-def intAddFunc [Coe String Ident] : LFunc Ident :=
+def intAddFunc : LFunc T :=
   binaryOp "Int.Add" .int
-  (some (binOpCeval Int Int LExpr.denoteInt Int.add .int))
+  (some (binOpCeval Int Int (LExpr.denoteInt T) Int.add .int))
 
-def intSubFunc [Coe String Ident] : LFunc Ident :=
+def intSubFunc : LFunc T :=
   binaryOp "Int.Sub" .int
-  (some (binOpCeval Int Int LExpr.denoteInt Int.sub .int))
+  (some (binOpCeval Int Int (LExpr.denoteInt T) Int.sub .int))
 
-def intMulFunc [Coe String Ident] : LFunc Ident :=
+def intMulFunc : LFunc T :=
   binaryOp "Int.Mul" .int
-  (some (binOpCeval Int Int LExpr.denoteInt Int.mul .int))
+  (some (binOpCeval Int Int (LExpr.denoteInt T) Int.mul .int))
 
-def intDivFunc [Coe String Ident] : LFunc Ident :=
+def intDivFunc : LFunc T :=
   binaryOp "Int.Div" .int
   (some cevalIntDiv)
 
-def intModFunc [Coe String Ident] : LFunc Ident :=
+def intModFunc : LFunc T :=
   binaryOp "Int.Mod" .int
   (some cevalIntMod)
 
-def intNegFunc [Coe String Ident] : LFunc Ident :=
+def intNegFunc : LFunc T :=
   unaryOp "Int.Neg" .int
-  (some (unOpCeval Int Int LExpr.denoteInt Int.neg .int))
+  (some (unOpCeval Int Int (LExpr.denoteInt T) Int.neg .int))
 
-def intLtFunc [Coe String Ident] : LFunc Ident :=
+def intLtFunc : LFunc T :=
   binaryPredicate "Int.Lt" .int
-  (some (binOpCeval Int Bool LExpr.denoteInt (fun x y => x < y) .bool))
+  (some (binOpCeval Int Bool (LExpr.denoteInt T) (fun x y => x < y) .bool))
 
-def intLeFunc [Coe String Ident] : LFunc Ident :=
+def intLeFunc : LFunc T :=
   binaryPredicate "Int.Le" .int
-  (some (binOpCeval Int Bool LExpr.denoteInt (fun x y => x <= y) .bool))
+  (some (binOpCeval Int Bool (LExpr.denoteInt T) (fun x y => x <= y) .bool))
 
-def intGtFunc [Coe String Ident] : LFunc Ident :=
+def intGtFunc : LFunc T :=
   binaryPredicate "Int.Gt" .int
-  (some (binOpCeval Int Bool LExpr.denoteInt (fun x y => x > y) .bool))
+  (some (binOpCeval Int Bool (LExpr.denoteInt T) (fun x y => x > y) .bool))
 
-def intGeFunc [Coe String Ident] : LFunc Ident :=
+def intGeFunc : LFunc T :=
   binaryPredicate "Int.Ge" .int
-  (some (binOpCeval Int Bool LExpr.denoteInt (fun x y => x >= y) .bool))
+  (some (binOpCeval Int Bool (LExpr.denoteInt T) (fun x y => x >= y) .bool))
 
 /- Boolean Operations -/
-def boolAndFunc [Coe String Ident] : LFunc Ident :=
+def boolAndFunc : LFunc T :=
   binaryOp "Bool.And" .bool
-  (some (binOpCeval Bool Bool LExpr.denoteBool Bool.and .bool))
+  (some (binOpCeval Bool Bool (LExpr.denoteBool T) Bool.and .bool))
 
-def boolOrFunc [Coe String Ident] : LFunc Ident :=
+def boolOrFunc : LFunc T :=
   binaryOp "Bool.Or" .bool
-  (some (binOpCeval Bool Bool LExpr.denoteBool Bool.or .bool))
+  (some (binOpCeval Bool Bool (LExpr.denoteBool T) Bool.or .bool))
 
-def boolImpliesFunc [Coe String Ident] : LFunc Ident :=
+def boolImpliesFunc : LFunc T :=
   binaryOp "Bool.Implies" .bool
-  (some (binOpCeval Bool Bool LExpr.denoteBool (fun x y => ((not x) || y)) .bool))
+  (some (binOpCeval Bool Bool (LExpr.denoteBool T) (fun x y => ((not x) || y)) .bool))
 
-def boolEquivFunc [Coe String Ident] : LFunc Ident :=
+def boolEquivFunc : LFunc T :=
   binaryOp "Bool.Equiv" .bool
-  (some (binOpCeval Bool Bool LExpr.denoteBool (fun x y => (x == y)) .bool))
+  (some (binOpCeval Bool Bool (LExpr.denoteBool T) (fun x y => (x == y)) .bool))
 
-def boolNotFunc [Coe String Ident] : LFunc Ident :=
+def boolNotFunc : LFunc T :=
   unaryOp "Bool.Not" .bool
-  (some (unOpCeval Bool Bool LExpr.denoteBool Bool.not .bool))
+  (some (unOpCeval Bool Bool (LExpr.denoteBool T) Bool.not .bool))
 
-def IntBoolFactory : @Factory String :=
+def IntBoolFactory : @Factory T :=
   open LTy.Syntax in #[
     intAddFunc,
     intSubFunc,
