Strata/DL/Lambda/LExprEval.lean
@@ -19,13 +19,19 @@ open Std (ToFormat Format format)
 
 namespace LExpr
 
-variable {Identifier : Type} [DecidableEq Identifier] [ToFormat Identifier]
+variable {T : LExprParams} [BEq T.Metadata] [DecidableEq T.Metadata] [ToFormat T.Metadata]
+         [Inhabited T.Identifier] [BEq T.Identifier] [DecidableEq T.Identifier] [ToFormat T.Identifier] [Traceable EvalProvenance T.Metadata]
+
+inductive EvalProvenance
+  | Original -- The metadata of the original expression
+  | ReplacementVar -- The original bound variable that was replaced
+  | Abstraction -- The lambda that triggered the replacement
 
 /--
 Check for boolean equality of two expressions `e1` and `e2` after erasing any
 type annotations.
 -/
-def eqModuloTypes (e1 e2 : (LExpr LMonoTy Identifier)) : Bool :=
+def eqModuloTypes (e1 e2 : (LExpr T.mono)) : Bool :=
   e1.eraseTypes == e2.eraseTypes
 
 /--
@@ -34,16 +40,15 @@ Canonical values of `LExpr`s.
 Equality is simply `==` (or more accurately, `eqModuloTypes`) for these
 `LExpr`s. Also see `eql` for a version that can tolerate nested metadata.
 -/
-def isCanonicalValue (e : (LExpr LMonoTy Identifier)) : Bool :=
+def isCanonicalValue (e : (LExpr T.mono)) : Bool :=
   match e with
-  | .const _ _ => true
-  | .abs _ _ =>
+  | .const _ _ _ => true
+  | .abs _ _ _ =>
     -- We're using the locally nameless representation, which guarantees that
     -- `closed (.abs e) = closed e` (see theorem `closed_abs`).
     -- So we could simplify the following to `closed e`, but leave it as is for
     -- clarity.
     LExpr.closed e
-  | .mdata _ e' => isCanonicalValue e'
   | _ => false
 
 /--
@@ -51,16 +56,11 @@ Equality of canonical values `e1` and `e2`.
 
 We can tolerate nested metadata here.
 -/
-def eql (e1 e2 : (LExpr LMonoTy Identifier))
+def eql (e1 e2 : (LExpr T.mono))
   (_h1 : isCanonicalValue e1) (_h2 : isCanonicalValue e2) : Bool :=
-  if eqModuloTypes e1 e2 then
-    true
-  else
-    let e1' := removeAllMData e1
-    let e2' := removeAllMData e2
-    eqModuloTypes e1' e2'
+  eqModuloTypes e1 e2
 
-instance : ToFormat (Except Format (LExpr LMonoTy Identifier)) where
+instance : ToFormat (Except Format (LExpr T.mono)) where
   format x := match x with
               | .ok e => format e
               | .error err => err
@@ -71,13 +71,13 @@ eta-expansion.
 
 E.g., `mkAbsOfArity 2 core` will give `λxλy ((core y) x)`.
 -/
-def mkAbsOfArity (arity : Nat) (core : (LExpr LMonoTy Identifier)) : (LExpr LMonoTy Identifier) :=
+def mkAbsOfArity (arity : Nat) (core : (LExpr T.mono)) : (LExpr T.mono) :=
   go 0 arity core
-  where go (bvarcount arity : Nat) (core : (LExpr LMonoTy Identifier)) : (LExpr LMonoTy Identifier) :=
+  where go (bvarcount arity : Nat) (core : (LExpr T.mono)) : (LExpr T.mono) :=
   match arity with
   | 0 => core
   | n + 1 =>
-    go (bvarcount + 1) n (.abs .none (.app core (.bvar bvarcount)))
+    go (bvarcount + 1) n (.abs core.metadata .none (.app core.metadata core (.bvar core.metadata bvarcount)))
 
 mutual
 /--
@@ -91,7 +91,8 @@ We prefer Curry-style semantics because they separate the type system from
 evaluation, allowing us to potentially apply different type systems with our
 expressions, along with supporting dynamically-typed languages.
 -/
-def eval (n : Nat) (σ : (LState Identifier)) (e : (LExpr LMonoTy Identifier)) : (LExpr LMonoTy Identifier) :=
+partial def eval (n : Nat) (σ : LState T) (e : LExpr T.mono) : LExpr T.mono :=
+  -- FIXME: Remove partial keyword once https://github.com/leanprover/lean4/issues/10353 is fixed
   match n with
   | 0 => e
   | n' + 1 =>
@@ -109,8 +110,8 @@ def eval (n : Nat) (σ : (LState Identifier)) (e : (LExpr LMonoTy Identifier)) :
           let new_e := substFvars body input_map
           eval n' σ new_e
         else
-          let new_e := mkApp op_expr args
-          if args.all isConst then
+          let new_e := @mkApp T.mono e.metadata op_expr args
+          if args.all (isConst T.mono) then
             -- All arguments in the function call are concrete.
             -- We can, provided a denotation function, evaluate this function
             -- call.
@@ -123,27 +124,25 @@ def eval (n : Nat) (σ : (LState Identifier)) (e : (LExpr LMonoTy Identifier)) :
         -- Not a call of a factory function.
         evalCore n' σ e
 
-def evalCore (n' : Nat) (σ : (LState Identifier)) (e : (LExpr LMonoTy Identifier)) : (LExpr LMonoTy Identifier) :=
+partial def evalCore  (n' : Nat) (σ : LState T) (e : LExpr T.mono) : LExpr T.mono :=
   match e with
-  | .const _ _  => e
-  | .op _ _     => e
-  | .bvar _     => e
-  | .fvar x ty  => (σ.state.findD x (ty, e)).snd
-   -- (FIXME): Perform metadata transform instead of erasing it here.
-  | .mdata _ e' => eval n' σ e'
+  | .const _ _ _  => e
+  | .op _ _ _     => e
+  | .bvar _ _     => e
+  | .fvar _ x ty  => (σ.state.findD x (ty, e)).snd
    -- Note: closed .abs terms are canonical values; we'll be here if .abs
    -- contains free variables.
-  | .abs _ _   => substFvarsFromState σ e
-  | .quant _ _ _ _ => substFvarsFromState σ e
-  | .app e1 e2 => evalApp n' σ e e1 e2
-  | .eq  e1 e2 => evalEq n' σ e1 e2
-  | .ite c t f => evalIte n' σ c t f
+  | .abs _ _ _   => LExpr.substFvarsFromState σ e
+  | .quant _ _ _ _ _ => LExpr.substFvarsFromState σ e
+  | .app _ e1 e2 => evalApp n' σ e e1 e2
+  | .eq m e1 e2 => evalEq n' σ m e1 e2
+  | .ite m c t f => evalIte n' σ m c t f
 
-def evalIte (n' : Nat) (σ : (LState Identifier)) (c t f : (LExpr LMonoTy Identifier)) : (LExpr LMonoTy Identifier) :=
+partial def evalIte (n' : Nat) (σ : LState T) (m: T.Metadata) (c t f : LExpr T.mono) : LExpr T.mono :=
   let c' := eval n' σ c
   match c' with
-  | .const "true" _ => eval n' σ t
-  | .const "false" _ => eval n' σ f
+  | .const _ "true" _ => eval n' σ t
+  | .const _ "false" _ => eval n' σ f
   | _ =>
     -- It's important to at least substitute `.fvar`s in both branches of the
     -- `ite` here so that we can replace the variables by the values in the
@@ -153,40 +152,45 @@ def evalIte (n' : Nat) (σ : (LState Identifier)) (c t f : (LExpr LMonoTy Identi
     -- let f' := eval n' σ f
     let t' := substFvarsFromState σ t
     let f' := substFvarsFromState σ f
-    ite c' t' f'
+    .ite m c' t' f'
 
-def evalEq (n' : Nat) (σ : (LState Identifier)) (e1 e2 : (LExpr LMonoTy Identifier)) : (LExpr LMonoTy Identifier) :=
+partial def evalEq (n' : Nat) (σ : LState T) (m: T.Metadata) (e1 e2 : LExpr T.mono) : LExpr T.mono :=
   open LTy.Syntax in
   let e1' := eval n' σ e1
   let e2' := eval n' σ e2
   if eqModuloTypes e1' e2' then
     -- Short-circuit: e1' and e2' are syntactically the same after type erasure.
-    LExpr.true
+    LExpr.true T m
   else if h: isCanonicalValue e1' ∧ isCanonicalValue e2' then
       if eql e1' e2' h.left h.right then
-        LExpr.true
-      else LExpr.false
+        LExpr.true T m
+      else LExpr.false T m
   else
-    .eq e1' e2'
+    .eq m e1' e2'
 
-def evalApp (n' : Nat) (σ : (LState Identifier)) (e e1 e2 : (LExpr LMonoTy Identifier)) : (LExpr LMonoTy Identifier) :=
+partial def evalApp (n' : Nat) (σ : LState T) (e e1 e2 : LExpr T.mono) : LExpr T.mono :=
   let e1' := eval n' σ e1
   let e2' := eval n' σ e2
   match e1' with
-  | .abs _ e1' =>
-    let e' := subst e2' e1'
+  | .abs mAbs _ e1' =>
+    let replacer := fun (replacementVar: T.Metadata) =>
+     (@LExpr.replaceMetadata (T := T.mono) (
+      Traceable.combine
+      [(EvalProvenance.Original,       e2'.metadata),
+       (EvalProvenance.ReplacementVar, replacementVar),
+       (EvalProvenance.Abstraction,    mAbs)]) e2');
+    let e' := subst replacer e1'
     if eqModuloTypes e e' then e else eval n' σ e'
-  | .op fn _ =>
+  | .op m fn _ =>
     match σ.config.factory.getFactoryLFunc fn with
-    | none => LExpr.app e1' e2'
-    | some lfunc =>
-      let e' := LExpr.app e1' e2'
+    | none => .app m e1' e2'
+    | some lfunc2 =>
+      let e' := LExpr.app m e1' e2'
       -- In `e'`, we have already supplied one input to `fn`.
       -- Note that we can't have 0-arity Factory functions at this point.
-      let e'' := mkAbsOfArity (lfunc.inputs.length - 1) e'
+      let e'' := @mkAbsOfArity T (lfunc2.inputs.length - 1) (e' : LExpr T.mono)
       eval n' σ e''
-  | _ => LExpr.app e1' e2'
-
+  | _ => .app e.metadata e1' e2'
 end
 
 end LExpr
