Strata/DL/Lambda/LState.lean
@@ -16,7 +16,7 @@ namespace Lambda
 
 open Std (ToFormat Format format)
 
-variable {Identifier : Type} [DecidableEq Identifier] [ToFormat Identifier]
+variable {T : LExprParams} [Inhabited T.Metadata] [BEq T.Metadata] [DecidableEq T.Identifier] [BEq T.Identifier] [ToFormat T.Identifier] [ToFormat (LFunc T)] [ToFormat (Scopes T)] [Inhabited (LExpr T.mono)]
 ---------------------------------------------------------------------
 
 /-
@@ -28,13 +28,13 @@ We rely on the parser disallowing Lambda variables to begin with `$__`, which is
 reserved for internal use. Also see `TEnv.genExprVar` used during type inference
 and `LState.genVar` used during evaluation.
 -/
-structure EvalConfig (Identifier : Type) where
-  factory : @Factory Identifier
+structure EvalConfig (T : LExprParams) where
+  factory : @Factory T
   fuel : Nat := 200
   varPrefix : String := "$__"
   gen : Nat := 0
 
-instance : ToFormat (EvalConfig Identifier) where
+instance : ToFormat (EvalConfig T) where
   format c :=
     f!"Eval Depth: {(repr c.fuel)}" ++ Format.line ++
     f!"Variable Prefix: {c.varPrefix}" ++ Format.line ++
@@ -42,15 +42,15 @@ instance : ToFormat (EvalConfig Identifier) where
     f!"Factory Functions:" ++ Format.line ++
     Std.Format.joinSep c.factory.toList f!"{Format.line}"
 
-def EvalConfig.init : (EvalConfig Identifier) :=
-  { factory := @Factory.default Identifier,
+def EvalConfig.init : (EvalConfig T) :=
+  { factory := @Factory.default T,
     fuel := 200,
     gen := 0 }
 
-def EvalConfig.incGen (c : (EvalConfig Identifier)) : (EvalConfig Identifier) :=
+def EvalConfig.incGen (c : (EvalConfig T)) : (EvalConfig T) :=
     { c with gen := c.gen + 1 }
 
-def EvalConfig.genSym (x : String) (c : (EvalConfig String)) : String × (EvalConfig String) :=
+def EvalConfig.genSym (x : String) (c : (EvalConfig T)) : String × (EvalConfig T) :=
   let new_idx := c.gen
   let c := c.incGen
   let new_var := c.varPrefix ++ x ++ toString new_idx
@@ -59,24 +59,24 @@ def EvalConfig.genSym (x : String) (c : (EvalConfig String)) : String × (EvalCo
 ---------------------------------------------------------------------
 
 /-- The Lambda evaluation state. -/
-structure LState (Identifier : Type) where
-  config : (EvalConfig Identifier)
-  state : (Scopes Identifier)
+structure LState (T : LExprParams) where
+  config : (EvalConfig T)
+  state : (Scopes T)
 
 -- scoped notation (name := lstate) "Σ" => LState
 
-def LState.init : (LState Identifier) :=
+def LState.init : (LState T) :=
   { state := [],
     config := EvalConfig.init }
 
 /-- An empty `LState` -/
-instance : EmptyCollection (LState Identifier) where
+instance : EmptyCollection (LState T) where
   emptyCollection := LState.init
 
-instance : Inhabited (LState Identifier) where
+instance : Inhabited (LState T) where
   default := LState.init
 
-instance : ToFormat (LState Identifier) where
+instance : ToFormat (LState T) where
   format s :=
     let { state, config }  := s
     format f!"State:{Format.line}{state}{Format.line}{Format.line}\
@@ -87,7 +87,7 @@ instance : ToFormat (LState Identifier) where
 Add function `func` to the existing factory of functions in `σ`. Redefinitions
 are not allowed.
 -/
-def LState.addFactoryFunc (σ : LState Identifier) (func : (LFunc Identifier)) : Except Format (LState Identifier) := do
+def LState.addFactoryFunc (σ : LState T) (func : (LFunc T)) : Except Format (LState T) := do
   let F ← σ.config.factory.addFactoryFunc func
   .ok { σ with config := { σ.config with factory := F }}
 
@@ -95,7 +95,7 @@ def LState.addFactoryFunc (σ : LState Identifier) (func : (LFunc Identifier)) :
 Append `Factory f` to the existing factory of functions in `σ`, checking for
 redefinitions.
 -/
-def LState.addFactory (σ : (LState Identifier)) (F : @Factory Identifier) : Except Format (LState Identifier) := do
+def LState.addFactory (σ : (LState T)) (F : @Factory T) : Except Format (LState T) := do
   let oldF := σ.config.factory
   let newF ← oldF.addFactory F
   .ok { σ with config := { σ.config with factory := newF } }
@@ -103,9 +103,9 @@ def LState.addFactory (σ : (LState Identifier)) (F : @Factory Identifier) : Exc
 /--
 Get all the known variables from the scopes in state `σ`.
 -/
-def LState.knownVars (σ : (LState Identifier)) : List Identifier :=
+def LState.knownVars (σ : (LState T)) : List T.Identifier :=
   go σ.state []
-  where go (s : Scopes Identifier) (acc : List Identifier) :=
+  where go (s : Scopes T) (acc : List T.Identifier) :=
   match s with
   | [] => acc
   | m :: rest => go rest (acc ++ m.keys)
@@ -114,30 +114,30 @@ def LState.knownVars (σ : (LState Identifier)) : List Identifier :=
 Generate a fresh (internal) identifier with the base name
 `x`; i.e., `σ.config.varPrefix ++ x`.
 -/
-def LState.genVar (x : String) (σ : (LState String)) : (String × (LState String)) :=
+def LState.genVar (x : String) (σ : (LState ⟨Metadata, String⟩)) : (String × (LState ⟨Metadata, String⟩)) :=
   let (new_var, config) := σ.config.genSym x
   let σ := { σ with config := config }
-  let known_vars := LState.knownVars σ
+  let known_vars : List String := LState.knownVars σ
   if new_var ∈ known_vars then
     panic s!"[LState.genVar] Generated variable {new_var} is not fresh!\n\
-             Known variables: {σ.knownVars}"
+             Known variables: {known_vars}"
   else
     (new_var, σ)
 
 /--
 Generate fresh identifiers, each with the base name in `xs`.
 -/
-def LState.genVars (xs : List String) (σ : (LState String)) : (List String × (LState String)) :=
+def LState.genVars (xs : List String) (σ : (LState ⟨Metadata, String⟩)) : (List String × (LState ⟨Metadata, String⟩)) :=
   let (vars, σ') := go xs σ []
   (vars.reverse, σ')
-  where go (xs : List String) (σ : LState String) (acc : List String) :=
+  where go (xs : List String) (σ : LState ⟨Metadata, String⟩) (acc : List String) :=
     match xs with
     | [] => (acc, σ)
     | x :: rest =>
       let (x', σ) := LState.genVar x σ
       go rest σ (x' :: acc)
 
-instance : ToFormat (Identifier × LState Identifier) where
+instance : ToFormat (T.Identifier × LState T) where
   format im :=
     f!"New Variable: {im.fst}{Format.line}\
        Gen in EvalConfig: {im.snd.config.gen}{Format.line}\
@@ -148,7 +148,7 @@ instance : ToFormat (Identifier × LState Identifier) where
 /--
 Substitute `.fvar`s in `e` by looking up their values in `σ`.
 -/
-def LExpr.substFvarsFromState (σ : (LState Identifier)) (e : (LExpr LMonoTy Identifier)) : (LExpr LMonoTy Identifier) :=
+def LExpr.substFvarsFromState (σ : (LState T)) (e : (LExpr T.mono)) : (LExpr T.mono) :=
   let sm := σ.state.toSingleMap.map (fun (x, (_, v)) => (x, v))
   Lambda.LExpr.substFvars e sm
 
